JaIris.v
@@ -330,6 +330,11 @@ Inductive JFIProves : JFIDeclsType -> JFITypeEnv -> JFITerm -> JFITerm -> Prop :
 
 (* Rules for separation logic *)
 
+| JFIWeakRule :
+    forall decls gamma p1 p2,
+      (*------------------------------------*)
+      JFIProves decls gamma (JFISep p1 p2) p1
+
 | JFISepAssoc1Rule :
     forall decls gamma p1 p2 p3,
       (*------------------------------------------------------------------*)
